\documentclass[11pt]{preprint}

\setlength{\topmargin}{0mm} \setlength{\oddsidemargin}{0mm}
\setlength{\textwidth}{160mm} \setlength{\textheight}{215mm}

\usepackage{amssymb,amsmath,amscd,amsthm}
\usepackage{graphics}
\usepackage{tikz}

\def\enumb{\begin{enumerate}}
\def\enume{\end{enumerate}}
\def\itemb{\begin{itemize}}
\def\iteme{\end{itemize}}
\def\integers{\mathbb{Z}}

\def\multiset#1#2{\ensuremath{\left(\kern-.3em\left(\genfrac{}{}{0pt}{}{#1}{#2}\right)\kern-.3em\right)}}



\newtheorem{proposition}{Proposition}
\newtheorem{theorem}{Theorem}
\newtheorem*{solution}{Solution}

\title{Discrete Mathematics, 2016 Fall - Worksheet 13}
\author{Instructor: Zsolt Pajor-Gyulai, CIMS}

\date{October 26, 2016}



\begin{document}

\maketitle

In all of the above problems explain your answer in full English sentences.
\enumb

\item Prove the following proposition.

\begin{proposition}
Let $a,b,$ and $c$ be sequences of numbers and let $s$ be a number.
\begin{itemize}
\item If, for all $n$, $c_n=a_n+b_n$ then $\Delta c_n=\Delta a_n+\Delta b_n$.
\item If, for all $n$, $b_n=sa_n$, then $\Delta b_n=s\Delta a_n$
\end{itemize}
\end{proposition}

\begin{proof}
Textbook page 159.
\end{proof}

\item Each of the following sequences is generated by a polynomial expression. For each, find the polynomial expression that gives $a_n$.
\begin{itemize}
\item $1,6,17,34,57,86,121,162,209,262,\dots$
\begin{solution}
By writing out the differences, we see that $k=2$, while
\[
a_0=1, \qquad \Delta a_0=5,\qquad \Delta^2a_0=6
\]
and thus

\[
a_n=1\cdot\binom{n}{0}+5\binom{n}{1}+6\binom{n}{2}=1+5n+6\frac{n(n-1)}{2}=3n^2+2n+1
\]
\end{solution}
\item $6,5,6,9,14,21,30,41,54,69,\dots$.
\begin{solution}
Once again, $k=2$ and 
\[
a_0=6,\qquad \Delta a_0=-1,\qquad \Delta^2a_0=2
\]
and therefore
\[
a_n=6\cdot\binom{n}{0}-\binom{n}{1}+2\binom{n}{2}=6-n+n(n-1)=n^2-2n+6
\]
\end{solution}
\end{itemize}

\item Find a polynomial formula for $1^2+2^2+3^2+\dots n^2$.

\begin{solution}
Textbook page 162.
\end{solution}
\enume
\end{document}